{-# OPTIONS --cubical --safe --guardedness #-}

open import Cubical.Algebra.Ring

module UMIN.L00_Core.Logic.FPS_Assoc {â„“} (R : Ring â„“) where

open import Cubical.Foundations.Prelude
open import Cubical.Foundations.Function
open import Cubical.Data.Nat using (â„•; zero; suc; _âˆ¸_) renaming (_+_ to _+â„•_)
open import Cubical.Data.Nat.Properties using (+-comm; +-suc; injSuc; snotz)
open import Cubical.Data.Empty using (âŠ¥; elim) renaming (rec to âŠ¥-elim)
open import Cubical.Data.Nat.Order using (_â‰¤_; zero-â‰¤; â‰¤-refl)
open import UMIN.L00_Core.Logic.EquationEngine
open import UMIN.L00_Core.Algebra.FPS_Base R

-- ======================================================================
-- 1. æ¨™æº–ãƒ©ã‚¤ãƒ–ãƒ©ãƒª Ring ã¨éå»è³‡ç”£ã®ãƒ–ãƒªãƒƒã‚¸
-- ======================================================================
private
  Carrier : Type â„“
  Carrier = fst R

open RingStr (snd R) renaming
  ( _+_  to _+R_
  ; _Â·_  to _*R_
  ; 0r   to 0R
  ; 1r   to 1R
  ; +Assoc  to +R-assoc-std
  ; +Comm   to +R-comm
  ; Â·Assoc  to *R-assoc-std
  ; Â·DistR+ to R-distribÊ³
  ; Â·DistL+ to R-distribË¡
  )

+R-assoc : âˆ€ x y z â†’ (x +R y) +R z â‰¡ x +R (y +R z)
+R-assoc x y z = sym (+R-assoc-std x y z)

*R-assoc : âˆ€ x y z â†’ (x *R y) *R z â‰¡ x *R (y *R z)
*R-assoc x y z = sym (*R-assoc-std x y z)

finiteSum : (â„• â†’ Carrier) â†’ â„• â†’ Carrier
finiteSum f zero = f zero
finiteSum f (suc n) = finiteSum f n +R f (suc n)

-- ======================================================================
-- 2. è£œé¡Œç¾¤ & ãƒ©ã‚¹ãƒœã‚¹è¨ä¼
-- ======================================================================
abstract
  sum-plus-sum : âˆ€ n (f g : â„• â†’ Carrier) â†’ 
    finiteSum (Î» k â†’ f k +R g k) n â‰¡ finiteSum f n +R finiteSum g n
  sum-plus-sum zero f g = refl
  sum-plus-sum (suc n) f g = 
    finiteSum (Î» k â†’ f k +R g k) n +R (f (suc n) +R g (suc n))
    â‰¡âŸ¨ cong (Î» x â†’ x +R (f (suc n) +R g (suc n))) (sum-plus-sum n f g) âŸ©â‡’
      (finiteSum f n +R finiteSum g n) +R (f (suc n) +R g (suc n))
    â‰¡âŸ¨ +R-assoc (finiteSum f n) (finiteSum g n) (f (suc n) +R g (suc n)) âŸ©â‡’
      finiteSum f n +R (finiteSum g n +R (f (suc n) +R g (suc n)))
    â‰¡âŸ¨ cong (Î» x â†’ finiteSum f n +R x) (sym (+R-assoc (finiteSum g n) (f (suc n)) (g (suc n)))) âŸ©â‡’
      finiteSum f n +R ((finiteSum g n +R f (suc n)) +R g (suc n))
    â‰¡âŸ¨ cong (Î» x â†’ finiteSum f n +R (x +R g (suc n))) (+R-comm (finiteSum g n) (f (suc n))) âŸ©â‡’
      finiteSum f n +R ((f (suc n) +R finiteSum g n) +R g (suc n))
    â‰¡âŸ¨ cong (Î» x â†’ finiteSum f n +R x) (+R-assoc (f (suc n)) (finiteSum g n) (g (suc n))) âŸ©â‡’
      finiteSum f n +R (f (suc n) +R (finiteSum g n +R g (suc n)))
    â‰¡âŸ¨ sym (+R-assoc (finiteSum f n) (f (suc n)) (finiteSum g n +R g (suc n))) âŸ©â‡’
      (finiteSum f n +R f (suc n)) +R (finiteSum g n +R g (suc n))
    âˆâ‡’

  finiteSum-ext : âˆ€ n (f g : â„• â†’ Carrier) â†’ (âˆ€ k â†’ k â‰¤ n â†’ f k â‰¡ g k) â†’ finiteSum f n â‰¡ finiteSum g n
  finiteSum-ext zero f g hyp = hyp zero zero-â‰¤
  finiteSum-ext (suc n) f g hyp = 
    congâ‚‚ _+R_ (finiteSum-ext n f g (Î» k kâ‰¤n â†’ hyp k (suc-â‰¤ kâ‰¤n))) 
               (hyp (suc n) â‰¤-refl)
    where
      suc-â‰¤ : âˆ€ {m n} â†’ m â‰¤ n â†’ m â‰¤ suc n
      suc-â‰¤ (k , p) = (suc k) , (cong suc p)

  jâ‰¤0â†’jâ‰¡0 : âˆ€ j â†’ j â‰¤ 0 â†’ j â‰¡ 0
  jâ‰¤0â†’jâ‰¡0 zero _ = refl
  jâ‰¤0â†’jâ‰¡0 (suc j) (k , p) = âŠ¥-elim (snotz (sym (+-comm k (suc j)) âˆ™ p))

  +-âˆ¸-assoc-lemma : âˆ€ i j â†’ j â‰¤ i â†’ j +â„• (i âˆ¸ j) â‰¡ i
  +-âˆ¸-assoc-lemma zero j jâ‰¤0 = cong (Î» x â†’ x +â„• (0 âˆ¸ x)) (jâ‰¤0â†’jâ‰¡0 j jâ‰¤0)
  +-âˆ¸-assoc-lemma (suc i) zero _ = refl
  +-âˆ¸-assoc-lemma (suc i) (suc j) (k , p) = cong suc (+-âˆ¸-assoc-lemma i j (k , lemma))
    where
      lemma : k +â„• j â‰¡ i
      lemma = injSuc (sym (+-suc k j) âˆ™ p)

  zeroâˆ¸ : âˆ€ m â†’ 0 âˆ¸ m â‰¡ 0
  zeroâˆ¸ zero = refl
  zeroâˆ¸ (suc m) = refl

  âˆ¸-dist-lemma : âˆ€ n k m â†’ n âˆ¸ (k +â„• m) â‰¡ (n âˆ¸ k) âˆ¸ m
  âˆ¸-dist-lemma n zero m = refl
  âˆ¸-dist-lemma zero (suc k) m = sym (zeroâˆ¸ m)
  âˆ¸-dist-lemma (suc n) (suc k) m = âˆ¸-dist-lemma n k m
  
  suc-âˆ¸-lemma : âˆ€ n k â†’ k â‰¤ n â†’ suc n âˆ¸ k â‰¡ suc (n âˆ¸ k)
  suc-âˆ¸-lemma n zero _ = refl
  suc-âˆ¸-lemma (suc n) (suc k) (x , p) = suc-âˆ¸-lemma n k (x , lemma-p)
    where
      lemma-p : x +â„• k â‰¡ n
      lemma-p = injSuc (sym (+-suc x k) âˆ™ p)
  suc-âˆ¸-lemma zero (suc k) (x , p) = âŠ¥-elim (snotz (sym (+-suc x k) âˆ™ p))

  nâˆ¸nâ‰¡0 : âˆ€ n â†’ n âˆ¸ n â‰¡ 0
  nâˆ¸nâ‰¡0 zero = refl
  nâˆ¸nâ‰¡0 (suc n) = nâˆ¸nâ‰¡0 n

  sum-distribÊ³-lemma : âˆ€ n (c : Carrier) (f : â„• â†’ Carrier) â†’ (finiteSum f n) *R c â‰¡ finiteSum (Î» k â†’ f k *R c) n
  sum-distribÊ³-lemma zero c f = refl
  sum-distribÊ³-lemma (suc n) c f =
    R-distribË¡ (finiteSum f n) (f (suc n)) c
    âˆ™ cong (Î» x â†’ x +R (f (suc n) *R c)) (sum-distribÊ³-lemma n c f)

  sum-distribË¡-lemma : âˆ€ n (c : Carrier) (f : â„• â†’ Carrier) â†’ c *R (finiteSum f n) â‰¡ finiteSum (Î» k â†’ c *R f k) n
  sum-distribË¡-lemma zero c f = refl
  sum-distribË¡-lemma (suc n) c f =
    R-distribÊ³ c (finiteSum f n) (f (suc n))
    âˆ™ cong (Î» x â†’ x +R (c *R f (suc n))) (sum-distribË¡-lemma n c f)

  double-sum-swap-lemma : (n : â„•) (F : â„• â†’ â„• â†’ Carrier) â†’ 
    finiteSum (Î» i â†’ finiteSum (Î» j â†’ F j (i âˆ¸ j)) i) n 
    â‰¡ finiteSum (Î» k â†’ finiteSum (Î» m â†’ F k m) (n âˆ¸ k)) n
  double-sum-swap-lemma zero F = refl
  double-sum-swap-lemma (suc n) F = 
    finiteSum (Î» i â†’ finiteSum (Î» j â†’ F j (i âˆ¸ j)) i) n 
    +R finiteSum (Î» j â†’ F j (suc n âˆ¸ j)) (suc n)
    â‰¡âŸ¨ cong (Î» x â†’ x +R finiteSum (Î» j â†’ F j (suc n âˆ¸ j)) (suc n)) (double-sum-swap-lemma n F) âŸ©â‡’
      finiteSum (Î» k â†’ finiteSum (Î» m â†’ F k m) (n âˆ¸ k)) n 
      +R finiteSum (Î» j â†’ F j (suc n âˆ¸ j)) (suc n)
    â‰¡âŸ¨ refl âŸ©â‡’
      finiteSum (Î» k â†’ finiteSum (Î» m â†’ F k m) (n âˆ¸ k)) n 
      +R (finiteSum (Î» j â†’ F j (suc n âˆ¸ j)) n +R F (suc n) (suc n âˆ¸ suc n))
    â‰¡âŸ¨ cong (Î» x â†’ finiteSum (Î» k â†’ finiteSum (Î» m â†’ F k m) (n âˆ¸ k)) n 
                     +R (finiteSum (Î» j â†’ F j (suc n âˆ¸ j)) n +R F (suc n) x)) 
             (nâˆ¸nâ‰¡0 (suc n)) âŸ©â‡’
      finiteSum (Î» k â†’ finiteSum (Î» m â†’ F k m) (n âˆ¸ k)) n 
      +R (finiteSum (Î» j â†’ F j (suc n âˆ¸ j)) n +R F (suc n) 0)
    â‰¡âŸ¨ sym (+R-assoc (finiteSum (Î» k â†’ finiteSum (Î» m â†’ F k m) (n âˆ¸ k)) n) 
                      (finiteSum (Î» j â†’ F j (suc n âˆ¸ j)) n) 
                      (F (suc n) 0)) âŸ©â‡’
      (finiteSum (Î» k â†’ finiteSum (Î» m â†’ F k m) (n âˆ¸ k)) n 
       +R finiteSum (Î» j â†’ F j (suc n âˆ¸ j)) n) 
      +R F (suc n) 0
    -- ğŸ’¡ ã“ã“ã§ _ _ ã‚’å®Œå…¨ã«é–¢æ•°åŒ–
    â‰¡âŸ¨ cong (Î» x â†’ x +R F (suc n) 0) (sym (sum-plus-sum n 
         (Î» k â†’ finiteSum (Î» m â†’ F k m) (n âˆ¸ k)) 
         (Î» k â†’ F k (suc n âˆ¸ k)))) âŸ©â‡’
      finiteSum (Î» k â†’ finiteSum (Î» m â†’ F k m) (n âˆ¸ k) +R F k (suc n âˆ¸ k)) n 
      +R F (suc n) 0
    -- ğŸ’¡ ã“ã“ã‚‚ _ _ ã‚’å®Œå…¨ã«é–¢æ•°åŒ–
    â‰¡âŸ¨ cong (Î» x â†’ x +R F (suc n) 0) (finiteSum-ext n 
         (Î» k â†’ finiteSum (Î» m â†’ F k m) (n âˆ¸ k) +R F k (suc n âˆ¸ k)) 
         (Î» k â†’ finiteSum (Î» m â†’ F k m) (n âˆ¸ k) +R F k (suc (n âˆ¸ k))) 
         (Î» k kâ‰¤n â†’ congâ‚‚ _+R_ refl (cong (F k) (suc-âˆ¸-lemma n k kâ‰¤n)))) âŸ©â‡’
      finiteSum (Î» k â†’ finiteSum (Î» m â†’ F k m) (n âˆ¸ k) +R F k (suc (n âˆ¸ k))) n 
      +R F (suc n) 0
    â‰¡âŸ¨ refl âŸ©â‡’
       finiteSum (Î» k â†’ finiteSum (Î» m â†’ F k m) (suc (n âˆ¸ k))) n 
       +R F (suc n) 0
    -- ğŸ’¡ ã“ã“ã‚‚ _ _ ã‚’å®Œå…¨ã«é–¢æ•°åŒ–
    â‰¡âŸ¨ cong (Î» x â†’ x +R F (suc n) 0) (finiteSum-ext n 
         (Î» k â†’ finiteSum (Î» m â†’ F k m) (suc (n âˆ¸ k))) 
         (Î» k â†’ finiteSum (Î» m â†’ F k m) (suc n âˆ¸ k)) 
         (Î» k kâ‰¤n â†’ cong (finiteSum (Î» m â†’ F k m)) (sym (suc-âˆ¸-lemma n k kâ‰¤n)))) âŸ©â‡’
       finiteSum (Î» k â†’ finiteSum (Î» m â†’ F k m) (suc n âˆ¸ k)) n 
       +R F (suc n) 0
    â‰¡âŸ¨ cong (Î» x â†’ finiteSum (Î» k â†’ finiteSum (Î» m â†’ F k m) (suc n âˆ¸ k)) n +R x) 
             (sym (cong (finiteSum (Î» m â†’ F (suc n) m)) (nâˆ¸nâ‰¡0 n))) âŸ©â‡’
       finiteSum (Î» k â†’ finiteSum (Î» m â†’ F k m) (suc n âˆ¸ k)) n 
       +R finiteSum (Î» m â†’ F (suc n) m) (n âˆ¸ n)
    â‰¡âŸ¨ refl âŸ©â‡’
       finiteSum (Î» k â†’ finiteSum (Î» m â†’ F k m) (suc n âˆ¸ k)) (suc n)
    âˆâ‡’

-- ======================================================================
-- 3. ğŸ’¥ æœ€çµ‚å®šç†ï¼šã‚¢ã‚½ã‚·ã‚¨ãƒ¼ã‚¿ Î¦ ã®ãƒ¡ã‚¤ãƒ³ãƒ‘ã‚¹
-- ======================================================================
FPS-Obj : Type â„“
FPS-Obj = FormalPowerSeries

open import Cubical.Algebra.Ring.BigOps using (module Sum)
open import Cubical.Data.FinData.Base
  using (Fin; toâ„•; weakenFin; fromâ„•; toFromId)
  renaming (zero to fzero; suc to fsuc)

open Sum R

distribRHS : FPS-Obj â†’ FPS-Obj â†’ FPS-Obj â†’ FPS-Obj
distribRHS A B C n =
  finiteSum (Î» i â†’
    finiteSum (Î» j â†’ (A j *R B (i âˆ¸ j)) *R C (n âˆ¸ i)) i) n

midRHS : FPS-Obj â†’ FPS-Obj â†’ FPS-Obj â†’ FPS-Obj
midRHS A B C n =
  finiteSum (Î» i â†’
    finiteSum (Î» j â†’ A j *R (B (i âˆ¸ j) *R C (n âˆ¸ i))) i) n

abstract
  -- ğŸ’¡ å®Œå…¨ã«å‹ã‚’æ˜ç¤ºã—ãŸ toâ„•-weakenFin
  toâ„•-weakenFin : âˆ€ {n} (k : Fin n) â†’ toâ„• (weakenFin k) â‰¡ toâ„• k
  toâ„•-weakenFin {n} k = Cubical.Data.FinData.Base.elim
    (Î» {m} (fn : Fin m) â†’ toâ„• (weakenFin fn) â‰¡ toâ„• fn)
    refl
    (Î» {m} {fn : Fin m} eq â†’ cong suc eq)
    k

  sum-bridge : âˆ€ n (f : â„• â†’ Carrier) â†’ 
    âˆ‘ {n = suc n} (Î» k â†’ f (toâ„• k)) â‰¡ finiteSum f n
  sum-bridge zero f =
    âˆ‘Last {n = 0} (Î» k â†’ f (toâ„• k))
    âˆ™ +IdL (f zero)
  sum-bridge (suc n) f =
    let
      V : Fin (suc (suc n)) â†’ Carrier
      V k = f (toâ„• k)
      pâ‚ : âˆ‘ V â‰¡ âˆ‘ (V âˆ˜ weakenFin) +R V (fromâ„• (suc n))
      pâ‚ = âˆ‘Last {n = suc n} V
      pTailAlign : âˆ‘ (V âˆ˜ weakenFin) â‰¡ âˆ‘ {n = suc n} (Î» k â†’ f (toâ„• k))
      pTailAlign = âˆ‘Ext {n = suc n} (Î» k â†’ cong f (toâ„•-weakenFin k))
      pâ‚‚ : âˆ‘ (V âˆ˜ weakenFin) â‰¡ finiteSum f n
      pâ‚‚ = pTailAlign âˆ™ sum-bridge n f
      step : âˆ‘ (V âˆ˜ weakenFin) +R V (fromâ„• (suc n)) â‰¡ âˆ‘ (V âˆ˜ weakenFin) +R f (suc n)
      step = cong (âˆ‘ (V âˆ˜ weakenFin) +R_) (cong f (toFromId (suc n)))
      pâ‚ƒ : âˆ‘ (V âˆ˜ weakenFin) +R f (suc n) â‰¡ finiteSum f n +R f (suc n)
      pâ‚ƒ = cong (Î» x â†’ x +R f (suc n)) pâ‚‚
    in
      pâ‚ âˆ™ step âˆ™ pâ‚ƒ

  âŠ—-finiteSum : âˆ€ (A B : FPS-Obj) n â†’
    (A âŠ— B) n â‰¡ finiteSum (Î» k â†’ A k *R B (n âˆ¸ k)) n
  âŠ—-finiteSum A B n = sum-bridge n (Î» k â†’ A k *R B (n âˆ¸ k))

  assoc-distrib : âˆ€ (A B C : FPS-Obj) â†’
    ((A âŠ— B) âŠ— C) â‰¡ distribRHS A B C
  assoc-distrib A B C = fps-ext Î» n â†’
    ((A âŠ— B) âŠ— C) n
    â‰¡âŸ¨ âŠ—-finiteSum (A âŠ— B) C n âŸ©â‡’
      finiteSum (Î» i â†’ (A âŠ— B) i *R C (n âˆ¸ i)) n
    â‰¡âŸ¨ cong (Î» F â†’ finiteSum F n) (funExt Î» i â†’ 
         cong (Î» X â†’ X *R C (n âˆ¸ i)) (âŠ—-finiteSum A B i)) âŸ©â‡’
      finiteSum (Î» i â†’ finiteSum (Î» j â†’ A j *R B (i âˆ¸ j)) i *R C (n âˆ¸ i)) n
    â‰¡âŸ¨ cong (Î» F â†’ finiteSum F n) (funExt Î» i â†’ 
         sum-distribÊ³-lemma i (C (n âˆ¸ i)) (Î» j â†’ A j *R B (i âˆ¸ j))) âŸ©â‡’
      distribRHS A B C n âˆâ‡’

  assoc-proof : âˆ€ (A B C : FPS-Obj) â†’
    distribRHS A B C â‰¡ midRHS A B C
  assoc-proof A B C = fps-ext Î» n â†’
    cong (Î» (F : â„• â†’ Carrier) â†’ finiteSum F n)
         (funExt Î» (i : â„•) â†’
           cong (Î» (G : â„• â†’ Carrier) â†’ finiteSum G i)
                (funExt Î» (j : â„•) â†’
                  *R-assoc (A j) (B (i âˆ¸ j)) (C (n âˆ¸ i))))

  assoc-block3 : âˆ€ (A B C : FPS-Obj) â†’
    midRHS A B C â‰¡ (A âŠ— (B âŠ— C))
  assoc-block3 A B C = fps-ext Î» n â†’
    midRHS A B C n
    -- ğŸ’¡ ã“ã“ã‚‚ _ _ ã‚’å®Œå…¨ã«é–¢æ•°åŒ–
    â‰¡âŸ¨ cong (Î» F â†’ finiteSum F n) (funExt Î» i â†’
         finiteSum-ext i 
           (Î» j â†’ A j *R (B (i âˆ¸ j) *R C (n âˆ¸ i))) 
           (Î» j â†’ A j *R (B (i âˆ¸ j) *R C (n âˆ¸ (j +â„• (i âˆ¸ j))))) 
           (Î» j jâ‰¤i â†’ cong (Î» X â†’ A j *R (B (i âˆ¸ j) *R C (n âˆ¸ X)))
                (sym (+-âˆ¸-assoc-lemma i j jâ‰¤i)))) âŸ©â‡’
      finiteSum (Î» i â†’ finiteSum (Î» j â†’ A j *R (B (i âˆ¸ j) *R C (n âˆ¸ (j +â„• (i âˆ¸ j))))) i) n
    â‰¡âŸ¨ double-sum-swap-lemma n (Î» k m â†’ A k *R (B m *R C (n âˆ¸ (k +â„• m)))) âŸ©â‡’
      finiteSum (Î» k â†’ finiteSum (Î» m â†’ A k *R (B m *R C (n âˆ¸ (k +â„• m)))) (n âˆ¸ k)) n
    â‰¡âŸ¨ cong (Î» F â†’ finiteSum F n) (funExt Î» k â†’
         sym (sum-distribË¡-lemma (n âˆ¸ k) (A k) (Î» m â†’ B m *R C (n âˆ¸ (k +â„• m))))) âŸ©â‡’
      finiteSum (Î» k â†’ A k *R finiteSum (Î» m â†’ B m *R C (n âˆ¸ (k +â„• m))) (n âˆ¸ k)) n
    â‰¡âŸ¨ cong (Î» F â†’ finiteSum F n) (funExt Î» k â†’
         cong (Î» X â†’ A k *R X)
         (cong (Î» G â†’ finiteSum G (n âˆ¸ k)) (funExt Î» m â†’
           cong (Î» Y â†’ B m *R C Y) (âˆ¸-dist-lemma n k m)))) âŸ©â‡’
      finiteSum (Î» k â†’ A k *R finiteSum (Î» m â†’ B m *R C ((n âˆ¸ k) âˆ¸ m)) (n âˆ¸ k)) n
    â‰¡âŸ¨ cong (Î» F â†’ finiteSum F n) (funExt Î» k â†’ 
         cong (Î» X â†’ A k *R X) (sym (âŠ—-finiteSum B C (n âˆ¸ k)))) âŸ©â‡’
      finiteSum (Î» k â†’ A k *R (B âŠ— C) (n âˆ¸ k)) n
    â‰¡âŸ¨ sym (âŠ—-finiteSum A (B âŠ— C) n) âŸ©â‡’
      (A âŠ— (B âŠ— C)) n âˆâ‡’

  FPS-Î±-proof : âˆ€ (A B C : FPS-Obj) â†’ 
    ((A âŠ— B) âŠ— C) â‰¡ (A âŠ— (B âŠ— C))
  FPS-Î±-proof A B C =
    assoc-distrib A B C âˆ™ assoc-proof A B C âˆ™ assoc-block3 A B C