{-# OPTIONS --cubical --guardedness #-}

-- ================================================================
-- Eâ‚ˆ Anomaly Cancellation Phase 2:
-- P/r Component Analysis & Zero Simplification Proofs
-- ================================================================
--
-- å®®ä¸‹å…ˆç”Ÿã®æŒ‡ç¤º:
--   ã€ŒÎ¦æˆåˆ†ã®å®‰å®šç¢ºèªã¯å®Œäº†ã€‚æ¬¡ã¯ã€Pæˆåˆ†ãŠã‚ˆã³ ræˆåˆ†ã«ãŠã‘ã‚‹
--    éè‡ªæ˜ãªç›¸æ®ºï¼ˆã‚«ã‚ªã‚¹ã®èª¿å¾‹ï¼‰ã«ç§»è¡Œã›ã‚ˆã€‚ã€
--
-- This file:
--   Â§A. Proves P-of-bracket-PQ etc. (removing postulates)
--   Â§B. Computes outer bracket P-components (where Ã—F-derivation acts)
--   Â§C. Analyzes r-component (where Î´ = 126/17 enters)
--
-- The key discovery: when two pure distortion elements bracket,
-- P and Q components vanish. But in the OUTER bracket, the
-- P-component picks up terms like E7-act(pâ‚‚ Ã—F pâ‚ƒ)(pâ‚) and
-- âŸ¨pâ‚‚,pâ‚ƒâŸ©âŠ›pâ‚ â€” THIS is where anomaly cancellation becomes
-- non-trivial and requires Ã—F-derivation to resolve.

module UMIN.L01_Math.Algebraic_Structures.LieAlgebra.E8AnomalyPhase2 where

open import Cubical.Foundations.Prelude
open import Cubical.Data.Nat using (â„•; zero; suc; _+_; _Â·_)

-- ================================================================
-- Â§0. Eâ‚‡ Interface (reproduced, self-contained)
-- ================================================================

record â„šâº : Type where
  constructor _//_
  field
    num : â„•
    den : â„•
open â„šâº

postulate
  E7  : Type
  Pá¶œ  : Type
  ğ•œ   : Type
  ğ•œ-zero  : ğ•œ
  ğ•œ-one   : ğ•œ
  _+ğ•œ_    : ğ•œ â†’ ğ•œ â†’ ğ•œ
  _Â·ğ•œ_    : ğ•œ â†’ ğ•œ â†’ ğ•œ
  -ğ•œ_     : ğ•œ â†’ ğ•œ

  [_,_]â‚‡     : E7 â†’ E7 â†’ E7
  E7-zero    : E7
  _+E7_      : E7 â†’ E7 â†’ E7
  -E7_       : E7 â†’ E7
  Bâ‚‡         : E7 â†’ E7 â†’ ğ•œ

  Pá¶œ-zero   : Pá¶œ
  _+P_      : Pá¶œ â†’ Pá¶œ â†’ Pá¶œ
  -P_       : Pá¶œ â†’ Pá¶œ
  _âŠ›P_     : ğ•œ â†’ Pá¶œ â†’ Pá¶œ

  E7-act    : E7 â†’ Pá¶œ â†’ Pá¶œ
  _Ã—F_      : Pá¶œ â†’ Pá¶œ â†’ E7
  âŸ¨_,_âŸ©â‚›   : Pá¶œ â†’ Pá¶œ â†’ ğ•œ
  _âŠ›E7_    : ğ•œ â†’ E7 â†’ E7

infixl 20 _+ğ•œ_ _+E7_ -E7_ _+P_ -P_
infixl 30 _Â·ğ•œ_ _âŠ›P_ _âŠ›E7_
infix  35 [_,_]â‚‡
infix  40 _Ã—F_

postulate
  -- Eâ‚‡ axioms
  E7-antisym : (Î¦â‚ Î¦â‚‚ : E7) â†’ [ Î¦â‚ , Î¦â‚‚ ]â‚‡ â‰¡ -E7 [ Î¦â‚‚ , Î¦â‚ ]â‚‡
  E7-Jacobi : (Î¦â‚ Î¦â‚‚ Î¦â‚ƒ : E7)
    â†’ (([ Î¦â‚ , [ Î¦â‚‚ , Î¦â‚ƒ ]â‚‡ ]â‚‡) +E7 ([ Î¦â‚‚ , [ Î¦â‚ƒ , Î¦â‚ ]â‚‡ ]â‚‡) +E7 ([ Î¦â‚ƒ , [ Î¦â‚ , Î¦â‚‚ ]â‚‡ ]â‚‡)) â‰¡ E7-zero
  E7-rep : (Î¦â‚ Î¦â‚‚ : E7) (P : Pá¶œ)
    â†’ E7-act [ Î¦â‚ , Î¦â‚‚ ]â‚‡ P â‰¡ (E7-act Î¦â‚ (E7-act Î¦â‚‚ P)) +P (-P (E7-act Î¦â‚‚ (E7-act Î¦â‚ P)))
  Ã—F-derivation : (Î¦ : E7) (P Q : Pá¶œ)
    â†’ [ Î¦ , P Ã—F Q ]â‚‡ â‰¡ ((E7-act Î¦ P) Ã—F Q) +E7 (P Ã—F (E7-act Î¦ Q))
  âŸ¨âŸ©-invariant : (Î¦ : E7) (P Q : Pá¶œ)
    â†’ âŸ¨ E7-act Î¦ P , Q âŸ©â‚› +ğ•œ âŸ¨ P , E7-act Î¦ Q âŸ©â‚› â‰¡ ğ•œ-zero
  âŸ¨âŸ©-antisym : (P Q : Pá¶œ) â†’ âŸ¨ P , Q âŸ©â‚› â‰¡ -ğ•œ âŸ¨ Q , P âŸ©â‚›
  Ã—F-antisym : (P Q : Pá¶œ) â†’ P Ã—F Q â‰¡ -E7 (Q Ã—F P)

  -- Algebraic laws
  +E7-assoc : (a b c : E7) â†’ (a +E7 b) +E7 c â‰¡ a +E7 (b +E7 c)
  +E7-comm  : (a b : E7) â†’ a +E7 b â‰¡ b +E7 a
  +E7-unitÊ³ : (a : E7) â†’ a +E7 E7-zero â‰¡ a
  +E7-unitË¡ : (a : E7) â†’ E7-zero +E7 a â‰¡ a
  +E7-invÊ³  : (a : E7) â†’ a +E7 (-E7 a) â‰¡ E7-zero
  +E7-invË¡  : (a : E7) â†’ (-E7 a) +E7 a â‰¡ E7-zero

  +P-assoc  : (a b c : Pá¶œ) â†’ (a +P b) +P c â‰¡ a +P (b +P c)
  +P-comm   : (a b : Pá¶œ) â†’ a +P b â‰¡ b +P a
  +P-unitË¡  : (a : Pá¶œ) â†’ Pá¶œ-zero +P a â‰¡ a
  +P-unitÊ³  : (a : Pá¶œ) â†’ a +P Pá¶œ-zero â‰¡ a
  +P-invË¡   : (a : Pá¶œ) â†’ (-P a) +P a â‰¡ Pá¶œ-zero
  +P-invÊ³   : (a : Pá¶œ) â†’ a +P (-P a) â‰¡ Pá¶œ-zero
  -P-zero   : -P Pá¶œ-zero â‰¡ Pá¶œ-zero

  âŠ›P-zero  : (p : Pá¶œ) â†’ ğ•œ-zero âŠ›P p â‰¡ Pá¶œ-zero
  âŠ›E7-zero : (Ï† : E7) â†’ ğ•œ-zero âŠ›E7 Ï† â‰¡ E7-zero

  E7-act-zero    : (Î¦ : E7) â†’ E7-act Î¦ Pá¶œ-zero â‰¡ Pá¶œ-zero
  E7-act-by-zero : (p : Pá¶œ) â†’ E7-act E7-zero p â‰¡ Pá¶œ-zero

  Ã—F-zeroË¡ : (q : Pá¶œ) â†’ Pá¶œ-zero Ã—F q â‰¡ E7-zero
  Ã—F-zeroÊ³ : (p : Pá¶œ) â†’ p Ã—F Pá¶œ-zero â‰¡ E7-zero

  âŸ¨âŸ©-zeroË¡ : (q : Pá¶œ) â†’ âŸ¨ Pá¶œ-zero , q âŸ©â‚› â‰¡ ğ•œ-zero
  âŸ¨âŸ©-zeroÊ³ : (p : Pá¶œ) â†’ âŸ¨ p , Pá¶œ-zero âŸ©â‚› â‰¡ ğ•œ-zero

  -E7-distrib-+E7 : (a b : E7) â†’ -E7 (a +E7 b) â‰¡ (-E7 a) +E7 (-E7 b)
  -E7-invol  : (a : E7) â†’ -E7 (-E7 a) â‰¡ a
  -E7-zero   : -E7 E7-zero â‰¡ E7-zero

  [,]â‚‡-zeroË¡ : (Î¦ : E7) â†’ [ E7-zero , Î¦ ]â‚‡ â‰¡ E7-zero
  [,]â‚‡-zeroÊ³ : (Î¦ : E7) â†’ [ Î¦ , E7-zero ]â‚‡ â‰¡ E7-zero

  +ğ•œ-unitË¡ : (x : ğ•œ) â†’ ğ•œ-zero +ğ•œ x â‰¡ x
  +ğ•œ-unitÊ³ : (x : ğ•œ) â†’ x +ğ•œ ğ•œ-zero â‰¡ x
  -ğ•œ-zero  : -ğ•œ ğ•œ-zero â‰¡ ğ•œ-zero


-- ================================================================
-- Â§1. Eâ‚ˆ Record and Bracket
-- ================================================================

record E8 : Type where
  constructor mkE8
  field
    Î¦ : E7 ; P : Pá¶œ ; Q : Pá¶œ ; r : ğ•œ ; u : ğ•œ ; v : ğ•œ
open E8

[_,_]â‚ˆ : E8 â†’ E8 â†’ E8
[ Râ‚ , Râ‚‚ ]â‚ˆ = mkE8 Î¦â€² Pâ€² Qâ€² râ€² uâ€² vâ€²
  where
    Î¦â‚ = Î¦ Râ‚ ; Î¦â‚‚ = Î¦ Râ‚‚ ; Pâ‚ = P Râ‚ ; Pâ‚‚ = P Râ‚‚ ; Qâ‚ = Q Râ‚ ; Qâ‚‚ = Q Râ‚‚
    râ‚ = r Râ‚ ; râ‚‚ = r Râ‚‚ ; uâ‚ = u Râ‚ ; uâ‚‚ = u Râ‚‚ ; vâ‚ = v Râ‚ ; vâ‚‚ = v Râ‚‚
    Î¦â€² = ([ Î¦â‚ , Î¦â‚‚ ]â‚‡) +E7 (Pâ‚ Ã—F Qâ‚‚) +E7 (-E7 (Pâ‚‚ Ã—F Qâ‚))
    Pâ€² = (E7-act Î¦â‚ Pâ‚‚) +P (-P (E7-act Î¦â‚‚ Pâ‚)) +P (râ‚ âŠ›P Pâ‚‚) +P (-P (râ‚‚ âŠ›P Pâ‚)) +P (uâ‚ âŠ›P Qâ‚‚) +P (-P (uâ‚‚ âŠ›P Qâ‚))
    Qâ€² = (E7-act Î¦â‚ Qâ‚‚) +P (-P (E7-act Î¦â‚‚ Qâ‚)) +P (-P (râ‚ âŠ›P Qâ‚‚)) +P (râ‚‚ âŠ›P Qâ‚) +P (vâ‚ âŠ›P Pâ‚‚) +P (-P (vâ‚‚ âŠ›P Pâ‚))
    râ€² = âŸ¨ Pâ‚ , Qâ‚‚ âŸ©â‚› +ğ•œ (-ğ•œ âŸ¨ Pâ‚‚ , Qâ‚ âŸ©â‚›)
    uâ€² = âŸ¨ Qâ‚ , Qâ‚‚ âŸ©â‚›
    vâ€² = âŸ¨ Pâ‚ , Pâ‚‚ âŸ©â‚›

infix 35 [_,_]â‚ˆ

E8-zero : E8
E8-zero = mkE8 E7-zero Pá¶œ-zero Pá¶œ-zero ğ•œ-zero ğ•œ-zero ğ•œ-zero

pureP : Pá¶œ â†’ E8
pureP p = mkE8 E7-zero p Pá¶œ-zero ğ•œ-zero ğ•œ-zero ğ•œ-zero

pureQ : Pá¶œ â†’ E8
pureQ q = mkE8 E7-zero Pá¶œ-zero q ğ•œ-zero ğ•œ-zero ğ•œ-zero


-- ================================================================
--     â•”â•â•â•â•â•â•â•â•â•â•â•â•â•â•â•â•â•â•â•â•â•â•â•â•â•â•â•â•â•â•â•â•â•â•â•â•â•â•â•â•â•â•â•â•â•â•â•â•â•â•â•—
--     â•‘  PART A: Zero Simplification Proofs              â•‘
--     â•‘  (Removing postulates from Phase 1)              â•‘
--     â•šâ•â•â•â•â•â•â•â•â•â•â•â•â•â•â•â•â•â•â•â•â•â•â•â•â•â•â•â•â•â•â•â•â•â•â•â•â•â•â•â•â•â•â•â•â•â•â•â•â•â•â•
-- ================================================================

-- ================================================================
-- Â§A.1  Helper: 6-fold Pá¶œ-zero simplification
-- ================================================================
-- The P-component of [pureP p, pureQ q]â‚ˆ expands to:
--
--   E7-act(0, 0) +P (-P(E7-act(0, p)))
--   +P (0 âŠ›P 0)  +P (-P(0 âŠ›P p))
--   +P (0 âŠ›P q)  +P (-P(0 âŠ›P 0))
--
-- where the arguments are:
--   Î¦â‚=0, Î¦â‚‚=0, Pâ‚=p, Pâ‚‚=0, Qâ‚=0, Qâ‚‚=q
--   râ‚=0, râ‚‚=0, uâ‚=0, uâ‚‚=0, vâ‚=0, vâ‚‚=0
--
-- Each of the 6 terms reduces to Pá¶œ-zero.

-- Individual term lemmas:
private
  -- E7-act(E7-zero, Pá¶œ-zero) = Pá¶œ-zero
  t1-PQ : (p q : Pá¶œ) â†’ E7-act E7-zero Pá¶œ-zero â‰¡ Pá¶œ-zero
  t1-PQ _ _ = E7-act-by-zero Pá¶œ-zero

  -- -P(E7-act(E7-zero, p)) = -P(Pá¶œ-zero) = Pá¶œ-zero
  t2-PQ : (p q : Pá¶œ) â†’ -P (E7-act E7-zero p) â‰¡ Pá¶œ-zero
  t2-PQ p _ = cong -P_ (E7-act-by-zero p) âˆ™ -P-zero

  -- ğ•œ-zero âŠ›P Pá¶œ-zero = Pá¶œ-zero
  t3-PQ : (p q : Pá¶œ) â†’ ğ•œ-zero âŠ›P Pá¶œ-zero â‰¡ Pá¶œ-zero
  t3-PQ _ _ = âŠ›P-zero Pá¶œ-zero

  -- -P(ğ•œ-zero âŠ›P p) = -P(Pá¶œ-zero) = Pá¶œ-zero
  t4-PQ : (p q : Pá¶œ) â†’ -P (ğ•œ-zero âŠ›P p) â‰¡ Pá¶œ-zero
  t4-PQ p _ = cong -P_ (âŠ›P-zero p) âˆ™ -P-zero

  -- ğ•œ-zero âŠ›P q = Pá¶œ-zero
  t5-PQ : (p q : Pá¶œ) â†’ ğ•œ-zero âŠ›P q â‰¡ Pá¶œ-zero
  t5-PQ _ q = âŠ›P-zero q

  -- -P(ğ•œ-zero âŠ›P Pá¶œ-zero) = Pá¶œ-zero
  t6-PQ : (p q : Pá¶œ) â†’ -P (ğ•œ-zero âŠ›P Pá¶œ-zero) â‰¡ Pá¶œ-zero
  t6-PQ _ _ = cong -P_ (âŠ›P-zero Pá¶œ-zero) âˆ™ -P-zero


-- Â§A.2  Chain collapse: sum of 6 zeros = zero
-- We need: 0 +P 0 +P 0 +P 0 +P 0 +P 0 = 0
-- Strategy: collapse from left, using +P-unitË¡ repeatedly.

six-zeros-P : Pá¶œ-zero +P Pá¶œ-zero +P Pá¶œ-zero +P Pá¶œ-zero +P Pá¶œ-zero +P Pá¶œ-zero â‰¡ Pá¶œ-zero
six-zeros-P =
    cong (_+P Pá¶œ-zero) (cong (_+P Pá¶œ-zero) (cong (_+P Pá¶œ-zero) (cong (_+P Pá¶œ-zero)
      (+P-unitË¡ Pá¶œ-zero))))
  âˆ™ cong (_+P Pá¶œ-zero) (cong (_+P Pá¶œ-zero) (cong (_+P Pá¶œ-zero)
      (+P-unitË¡ Pá¶œ-zero)))
  âˆ™ cong (_+P Pá¶œ-zero) (cong (_+P Pá¶œ-zero)
      (+P-unitË¡ Pá¶œ-zero))
  âˆ™ cong (_+P Pá¶œ-zero)
      (+P-unitË¡ Pá¶œ-zero)
  âˆ™ +P-unitË¡ Pá¶œ-zero


-- ================================================================
-- Â§A.3  THEOREM: P-of-bracket-PQ (previously postulated)
-- ================================================================
-- P [pureP p, pureQ q]â‚ˆ â‰¡ Pá¶œ-zero

P-of-bracket-PQ : (p q : Pá¶œ)
  â†’ P [ pureP p , pureQ q ]â‚ˆ â‰¡ Pá¶œ-zero
P-of-bracket-PQ p q =
  -- P [pureP p, pureQ q]â‚ˆ definitionally equals:
  -- E7-act(0, 0) +P (-P(E7-act(0, p))) +P (0âŠ›0) +P (-P(0âŠ›p)) +P (0âŠ›q) +P (-P(0âŠ›0))
  --
  -- Rewrite each of the 6 terms to Pá¶œ-zero, then collapse.
  congâ‚‚ (Î» a b â†’ a +P b +P (ğ•œ-zero âŠ›P Pá¶œ-zero) +P (-P (ğ•œ-zero âŠ›P p)) +P (ğ•œ-zero âŠ›P q) +P (-P (ğ•œ-zero âŠ›P Pá¶œ-zero)))
    (t1-PQ p q) (t2-PQ p q)
  âˆ™ congâ‚‚ (Î» a b â†’ Pá¶œ-zero +P Pá¶œ-zero +P a +P b +P (ğ•œ-zero âŠ›P q) +P (-P (ğ•œ-zero âŠ›P Pá¶œ-zero)))
      (t3-PQ p q) (t4-PQ p q)
  âˆ™ congâ‚‚ (Î» a b â†’ Pá¶œ-zero +P Pá¶œ-zero +P Pá¶œ-zero +P Pá¶œ-zero +P a +P b)
      (t5-PQ p q) (t6-PQ p q)
  âˆ™ six-zeros-P


-- ================================================================
-- Â§A.4  THEOREM: Q-of-bracket-PQ (previously postulated)
-- ================================================================
-- Q [pureP p, pureQ q]â‚ˆ
-- Q-component formula with Î¦â‚=0, Î¦â‚‚=0, Qâ‚=0, Qâ‚‚=q, Pâ‚=p, Pâ‚‚=0:
--   E7-act(0, q) +P (-P(E7-act(0, 0))) +P (-P(0âŠ›q)) +P (0âŠ›0)
--   +P (0âŠ›0) +P (-P(0âŠ›p))

private
  -- E7-act(E7-zero, q) = Pá¶œ-zero
  q1-PQ : (p q : Pá¶œ) â†’ E7-act E7-zero q â‰¡ Pá¶œ-zero
  q1-PQ _ q = E7-act-by-zero q

  -- -P(E7-act(E7-zero, Pá¶œ-zero)) = Pá¶œ-zero
  q2-PQ : (p q : Pá¶œ) â†’ -P (E7-act E7-zero Pá¶œ-zero) â‰¡ Pá¶œ-zero
  q2-PQ _ _ = cong -P_ (E7-act-by-zero Pá¶œ-zero) âˆ™ -P-zero

  -- -P(ğ•œ-zero âŠ›P q) = Pá¶œ-zero
  q3-PQ : (p q : Pá¶œ) â†’ -P (ğ•œ-zero âŠ›P q) â‰¡ Pá¶œ-zero
  q3-PQ _ q = cong -P_ (âŠ›P-zero q) âˆ™ -P-zero

  -- ğ•œ-zero âŠ›P Pá¶œ-zero = Pá¶œ-zero
  q4-PQ : (p q : Pá¶œ) â†’ ğ•œ-zero âŠ›P Pá¶œ-zero â‰¡ Pá¶œ-zero
  q4-PQ _ _ = âŠ›P-zero Pá¶œ-zero

  -- ğ•œ-zero âŠ›P Pá¶œ-zero = Pá¶œ-zero  (vâ‚ âŠ›P Pâ‚‚)
  q5-PQ : (p q : Pá¶œ) â†’ ğ•œ-zero âŠ›P Pá¶œ-zero â‰¡ Pá¶œ-zero
  q5-PQ _ _ = âŠ›P-zero Pá¶œ-zero

  -- -P(ğ•œ-zero âŠ›P p) = Pá¶œ-zero
  q6-PQ : (p q : Pá¶œ) â†’ -P (ğ•œ-zero âŠ›P p) â‰¡ Pá¶œ-zero
  q6-PQ p _ = cong -P_ (âŠ›P-zero p) âˆ™ -P-zero


Q-of-bracket-PQ : (p q : Pá¶œ)
  â†’ Q [ pureP p , pureQ q ]â‚ˆ â‰¡ Pá¶œ-zero
Q-of-bracket-PQ p q =
  congâ‚‚ (Î» a b â†’ a +P b +P (-P (ğ•œ-zero âŠ›P q)) +P (ğ•œ-zero âŠ›P Pá¶œ-zero) +P (ğ•œ-zero âŠ›P Pá¶œ-zero) +P (-P (ğ•œ-zero âŠ›P p)))
    (q1-PQ p q) (q2-PQ p q)
  âˆ™ congâ‚‚ (Î» a b â†’ Pá¶œ-zero +P Pá¶œ-zero +P a +P b +P (ğ•œ-zero âŠ›P Pá¶œ-zero) +P (-P (ğ•œ-zero âŠ›P p)))
      (q3-PQ p q) (q4-PQ p q)
  âˆ™ congâ‚‚ (Î» a b â†’ Pá¶œ-zero +P Pá¶œ-zero +P Pá¶œ-zero +P Pá¶œ-zero +P a +P b)
      (q5-PQ p q) (q6-PQ p q)
  âˆ™ six-zeros-P


-- ================================================================
-- Â§A.5  P,Q vanishing for [pureQ q, pureP p] and [pureP, pureP]
-- ================================================================
-- Same technique: expand, show each term is Pá¶œ-zero, collapse.
-- For [pureQ q, pureP p]: Î¦â‚=0, Î¦â‚‚=0, Pâ‚=0, Pâ‚‚=p, Qâ‚=q, Qâ‚‚=0
-- For [pureP pâ‚, pureP pâ‚‚]: Î¦â‚=0, Î¦â‚‚=0, Pâ‚=pâ‚, Pâ‚‚=pâ‚‚, Qâ‚=0, Qâ‚‚=0

P-of-bracket-QP : (q p : Pá¶œ)
  â†’ P [ pureQ q , pureP p ]â‚ˆ â‰¡ Pá¶œ-zero
P-of-bracket-QP q p =
  -- P-component: E7-act(0,p) +P (-P(E7-act(0,0))) +P (0âŠ›p) +P (-P(0âŠ›0)) +P (0âŠ›0) +P (-P(0âŠ›q))
  congâ‚‚ (Î» a b â†’ a +P b +P (ğ•œ-zero âŠ›P p) +P (-P (ğ•œ-zero âŠ›P Pá¶œ-zero)) +P (ğ•œ-zero âŠ›P Pá¶œ-zero) +P (-P (ğ•œ-zero âŠ›P q)))
    (E7-act-by-zero p) (cong -P_ (E7-act-by-zero Pá¶œ-zero) âˆ™ -P-zero)
  âˆ™ congâ‚‚ (Î» a b â†’ Pá¶œ-zero +P Pá¶œ-zero +P a +P b +P (ğ•œ-zero âŠ›P Pá¶œ-zero) +P (-P (ğ•œ-zero âŠ›P q)))
      (âŠ›P-zero p) (cong -P_ (âŠ›P-zero Pá¶œ-zero) âˆ™ -P-zero)
  âˆ™ congâ‚‚ (Î» a b â†’ Pá¶œ-zero +P Pá¶œ-zero +P Pá¶œ-zero +P Pá¶œ-zero +P a +P b)
      (âŠ›P-zero Pá¶œ-zero) (cong -P_ (âŠ›P-zero q) âˆ™ -P-zero)
  âˆ™ six-zeros-P


Q-of-bracket-QP : (q p : Pá¶œ)
  â†’ Q [ pureQ q , pureP p ]â‚ˆ â‰¡ Pá¶œ-zero
Q-of-bracket-QP q p =
  -- Q-component: E7-act(0,0) +P (-P(E7-act(0,q))) +P (-P(0âŠ›0)) +P (0âŠ›q) +P (0âŠ›p) +P (-P(0âŠ›0))
  congâ‚‚ (Î» a b â†’ a +P b +P (-P (ğ•œ-zero âŠ›P Pá¶œ-zero)) +P (ğ•œ-zero âŠ›P q) +P (ğ•œ-zero âŠ›P p) +P (-P (ğ•œ-zero âŠ›P Pá¶œ-zero)))
    (E7-act-by-zero Pá¶œ-zero) (cong -P_ (E7-act-by-zero q) âˆ™ -P-zero)
  âˆ™ congâ‚‚ (Î» a b â†’ Pá¶œ-zero +P Pá¶œ-zero +P a +P b +P (ğ•œ-zero âŠ›P p) +P (-P (ğ•œ-zero âŠ›P Pá¶œ-zero)))
      (cong -P_ (âŠ›P-zero Pá¶œ-zero) âˆ™ -P-zero) (âŠ›P-zero q)
  âˆ™ congâ‚‚ (Î» a b â†’ Pá¶œ-zero +P Pá¶œ-zero +P Pá¶œ-zero +P Pá¶œ-zero +P a +P b)
      (âŠ›P-zero p) (cong -P_ (âŠ›P-zero Pá¶œ-zero) âˆ™ -P-zero)
  âˆ™ six-zeros-P


P-of-bracket-PP : (pâ‚ pâ‚‚ : Pá¶œ)
  â†’ P [ pureP pâ‚ , pureP pâ‚‚ ]â‚ˆ â‰¡ Pá¶œ-zero
P-of-bracket-PP pâ‚ pâ‚‚ =
  -- Pâ‚=pâ‚, Pâ‚‚=pâ‚‚, Qâ‚=Qâ‚‚=0, all scalars 0
  -- P-component: E7-act(0,pâ‚‚) +P (-P(E7-act(0,pâ‚))) +P (0âŠ›pâ‚‚) +P (-P(0âŠ›pâ‚)) +P (0âŠ›0) +P (-P(0âŠ›0))
  congâ‚‚ (Î» a b â†’ a +P b +P (ğ•œ-zero âŠ›P pâ‚‚) +P (-P (ğ•œ-zero âŠ›P pâ‚)) +P (ğ•œ-zero âŠ›P Pá¶œ-zero) +P (-P (ğ•œ-zero âŠ›P Pá¶œ-zero)))
    (E7-act-by-zero pâ‚‚) (cong -P_ (E7-act-by-zero pâ‚) âˆ™ -P-zero)
  âˆ™ congâ‚‚ (Î» a b â†’ Pá¶œ-zero +P Pá¶œ-zero +P a +P b +P (ğ•œ-zero âŠ›P Pá¶œ-zero) +P (-P (ğ•œ-zero âŠ›P Pá¶œ-zero)))
      (âŠ›P-zero pâ‚‚) (cong -P_ (âŠ›P-zero pâ‚) âˆ™ -P-zero)
  âˆ™ congâ‚‚ (Î» a b â†’ Pá¶œ-zero +P Pá¶œ-zero +P Pá¶œ-zero +P Pá¶œ-zero +P a +P b)
      (âŠ›P-zero Pá¶œ-zero) (cong -P_ (âŠ›P-zero Pá¶œ-zero) âˆ™ -P-zero)
  âˆ™ six-zeros-P


Q-of-bracket-PP : (pâ‚ pâ‚‚ : Pá¶œ)
  â†’ Q [ pureP pâ‚ , pureP pâ‚‚ ]â‚ˆ â‰¡ Pá¶œ-zero
Q-of-bracket-PP pâ‚ pâ‚‚ =
  -- Qâ‚=Qâ‚‚=0, Pâ‚=pâ‚, Pâ‚‚=pâ‚‚
  -- Q-component: E7-act(0,0) +P (-P(E7-act(0,0))) +P (-P(0âŠ›0)) +P (0âŠ›0) +P (0âŠ›pâ‚‚) +P (-P(0âŠ›pâ‚))
  congâ‚‚ (Î» a b â†’ a +P b +P (-P (ğ•œ-zero âŠ›P Pá¶œ-zero)) +P (ğ•œ-zero âŠ›P Pá¶œ-zero) +P (ğ•œ-zero âŠ›P pâ‚‚) +P (-P (ğ•œ-zero âŠ›P pâ‚)))
    (E7-act-by-zero Pá¶œ-zero) (cong -P_ (E7-act-by-zero Pá¶œ-zero) âˆ™ -P-zero)
  âˆ™ congâ‚‚ (Î» a b â†’ Pá¶œ-zero +P Pá¶œ-zero +P a +P b +P (ğ•œ-zero âŠ›P pâ‚‚) +P (-P (ğ•œ-zero âŠ›P pâ‚)))
      (cong -P_ (âŠ›P-zero Pá¶œ-zero) âˆ™ -P-zero) (âŠ›P-zero Pá¶œ-zero)
  âˆ™ congâ‚‚ (Î» a b â†’ Pá¶œ-zero +P Pá¶œ-zero +P Pá¶œ-zero +P Pá¶œ-zero +P a +P b)
      (âŠ›P-zero pâ‚‚) (cong -P_ (âŠ›P-zero pâ‚) âˆ™ -P-zero)
  âˆ™ six-zeros-P


-- ================================================================
--     â•”â•â•â•â•â•â•â•â•â•â•â•â•â•â•â•â•â•â•â•â•â•â•â•â•â•â•â•â•â•â•â•â•â•â•â•â•â•â•â•â•â•â•â•â•â•â•â•â•â•â•â•—
--     â•‘  PART B: Outer Bracket P-Component Analysis      â•‘
--     â•‘  (Where Ã—F-derivation enters the picture)        â•‘
--     â•šâ•â•â•â•â•â•â•â•â•â•â•â•â•â•â•â•â•â•â•â•â•â•â•â•â•â•â•â•â•â•â•â•â•â•â•â•â•â•â•â•â•â•â•â•â•â•â•â•â•â•â•
-- ================================================================

-- ================================================================
-- Â§B.1  P-component of [pureP pâ‚, M]â‚ˆ  where M = [pureP pâ‚‚, pureQ pâ‚ƒ]â‚ˆ
-- ================================================================
--
-- M has: Î¦(M) = pâ‚‚ Ã—F pâ‚ƒ,  P(M) = 0,  Q(M) = 0,
--        r(M) = âŸ¨pâ‚‚,pâ‚ƒâŸ©â‚›,  u(M) = 0,  v(M) = 0
--
-- [pureP pâ‚, M]â‚ˆ P-component:
--   Î¦â‚ = 0, Î¦â‚‚ = pâ‚‚ Ã—F pâ‚ƒ
--   Pâ‚ = pâ‚, Pâ‚‚ = 0
--   Qâ‚ = 0, Qâ‚‚ = 0
--   râ‚ = 0, râ‚‚ = âŸ¨pâ‚‚,pâ‚ƒâŸ©â‚›
--   uâ‚ = 0, uâ‚‚ = 0
--   vâ‚ = 0, vâ‚‚ = 0
--
-- Pâ€² = E7-act(0, 0)                    -- term 1: 0
--      +P (-P(E7-act(pâ‚‚Ã—Fpâ‚ƒ, pâ‚)))    -- term 2: â˜… NON-ZERO
--      +P (0 âŠ›P 0)                     -- term 3: 0
--      +P (-P(âŸ¨pâ‚‚,pâ‚ƒâŸ©â‚› âŠ›P pâ‚))       -- term 4: â˜… NON-ZERO
--      +P (0 âŠ›P 0)                     -- term 5: 0
--      +P (-P(0 âŠ›P 0))                 -- term 6: 0
--
-- Simplified:
--   Pâ€² = -P(E7-act(pâ‚‚ Ã—F pâ‚ƒ)(pâ‚)) +P (-P(âŸ¨pâ‚‚,pâ‚ƒâŸ©â‚› âŠ›P pâ‚))
--
-- THIS is the non-trivial content:
--   Term A: Eâ‚‡ core (pâ‚‚ Ã—F pâ‚ƒ) rotating pâ‚ via adjoint action
--   Term B: Scalar coupling âŸ¨pâ‚‚,pâ‚ƒâŸ©â‚› scaling pâ‚
--
-- For the Jacobi identity on P-components, the cyclic sum of
-- three such expressions must vanish. This is where Ã—F-derivation
-- and the symplectic pairing âŸ¨âŸ©-invariant play their roles.

-- Type alias for readability
P-outer-1-expected : Pá¶œ â†’ Pá¶œ â†’ Pá¶œ â†’ Pá¶œ
P-outer-1-expected pâ‚ pâ‚‚ pâ‚ƒ =
  (-P (E7-act (pâ‚‚ Ã—F pâ‚ƒ) pâ‚)) +P (-P (âŸ¨ pâ‚‚ , pâ‚ƒ âŸ©â‚› âŠ›P pâ‚))


-- ================================================================
-- Â§B.2  Summary: Non-trivial P-components of outer brackets
-- ================================================================
--
-- Term 1: P[pureP pâ‚, [pureP pâ‚‚, pureQ pâ‚ƒ]â‚ˆ]â‚ˆ
--   = -P(E7-act(pâ‚‚ Ã—F pâ‚ƒ)(pâ‚)) +P (-P(âŸ¨pâ‚‚,pâ‚ƒâŸ©â‚› âŠ›P pâ‚))
--
-- Term 2: P[pureP pâ‚‚, [pureQ pâ‚ƒ, pureP pâ‚]â‚ˆ]â‚ˆ
--   Inner: Î¦ = -E7(pâ‚ Ã—F pâ‚ƒ),  r = âŸ¨0,pâ‚âŸ©â‚› - âŸ¨p,0âŸ©â‚› = ...
--   (More complex â€” requires careful tracking)
--
-- Term 3: P[pureQ pâ‚ƒ, [pureP pâ‚, pureP pâ‚‚]â‚ˆ]â‚ˆ
--   Inner: Î¦ = E7-zero, r = âŸ¨pâ‚,0âŸ©â‚› - âŸ¨pâ‚‚,0âŸ©â‚› = 0
--   (Simpler â€” Î¦=0 means no E7-act contribution)
--
-- The CYCLIC SUM of these three P-components must vanish.
-- This is where the real anomaly cancellation happens,
-- mediated by Ã—F-derivation and âŸ¨âŸ©-invariant.


-- ================================================================
--     â•”â•â•â•â•â•â•â•â•â•â•â•â•â•â•â•â•â•â•â•â•â•â•â•â•â•â•â•â•â•â•â•â•â•â•â•â•â•â•â•â•â•â•â•â•â•â•â•â•â•â•â•—
--     â•‘  PART C: r-Component & Î´ = 126/17 Connection     â•‘
--     â•šâ•â•â•â•â•â•â•â•â•â•â•â•â•â•â•â•â•â•â•â•â•â•â•â•â•â•â•â•â•â•â•â•â•â•â•â•â•â•â•â•â•â•â•â•â•â•â•â•â•â•â•
-- ================================================================

-- ================================================================
-- Â§C.1  r-component of inner brackets
-- ================================================================
--
-- [pureP p, pureQ q]â‚ˆ .r = âŸ¨p,qâŸ©â‚›         (proved in Phase 1)
-- [pureQ q, pureP p]â‚ˆ .r = âŸ¨0,0âŸ©â‚› - âŸ¨p,qâŸ©â‚› = -âŸ¨p,qâŸ©â‚›
-- [pureP pâ‚, pureP pâ‚‚]â‚ˆ .r = âŸ¨pâ‚,0âŸ©â‚› - âŸ¨pâ‚‚,0âŸ©â‚› = 0

r-of-bracket-QP : (q p : Pá¶œ)
  â†’ r [ pureQ q , pureP p ]â‚ˆ â‰¡ -ğ•œ âŸ¨ p , q âŸ©â‚›
r-of-bracket-QP q p =
  -- r = âŸ¨Pâ‚,Qâ‚‚âŸ©â‚› +ğ•œ (-ğ•œ âŸ¨Pâ‚‚,Qâ‚âŸ©â‚›)
  -- Pâ‚=Pá¶œ-zero, Qâ‚‚=Pá¶œ-zero, Pâ‚‚=p, Qâ‚=q
  -- = âŸ¨0,0âŸ©â‚› +ğ•œ (-ğ•œ âŸ¨p,qâŸ©â‚›)
  -- = 0 +ğ•œ (-ğ•œ âŸ¨p,qâŸ©â‚›)
  -- = -ğ•œ âŸ¨p,qâŸ©â‚›
  cong (_+ğ•œ (-ğ•œ âŸ¨ p , q âŸ©â‚›)) (âŸ¨âŸ©-zeroË¡ Pá¶œ-zero)
  âˆ™ +ğ•œ-unitË¡ (-ğ•œ âŸ¨ p , q âŸ©â‚›)


r-of-bracket-PP : (pâ‚ pâ‚‚ : Pá¶œ)
  â†’ r [ pureP pâ‚ , pureP pâ‚‚ ]â‚ˆ â‰¡ ğ•œ-zero
r-of-bracket-PP pâ‚ pâ‚‚ =
  -- r = âŸ¨pâ‚,0âŸ©â‚› +ğ•œ (-ğ•œ âŸ¨pâ‚‚,0âŸ©â‚›)
  -- = 0 +ğ•œ (-ğ•œ 0)
  -- = 0 +ğ•œ 0 = 0
  congâ‚‚ (Î» a b â†’ a +ğ•œ (-ğ•œ b)) (âŸ¨âŸ©-zeroÊ³ pâ‚) (âŸ¨âŸ©-zeroÊ³ pâ‚‚)
  âˆ™ cong (ğ•œ-zero +ğ•œ_) -ğ•œ-zero
  âˆ™ +ğ•œ-unitË¡ ğ•œ-zero


-- ================================================================
-- Â§C.2  The distortion factor in context
-- ================================================================
--
-- The r-component of the outer bracket [pureP pâ‚, M]â‚ˆ where
-- M = [pureP pâ‚‚, pureQ pâ‚ƒ]â‚ˆ is:
--
--   râ€² = âŸ¨pâ‚, Q(M)âŸ©â‚› +ğ•œ (-ğ•œ âŸ¨P(M), 0âŸ©â‚›)
--      = âŸ¨pâ‚, 0âŸ©â‚› +ğ•œ (-ğ•œ âŸ¨0, 0âŸ©â‚›)   (since P(M)=Q(M)=0)
--      = 0
--
-- So the r-component of each outer double bracket also vanishes!
-- The scalar coupling âŸ¨pâ‚‚,pâ‚ƒâŸ©â‚› from the inner bracket enters
-- only through the P-component (as âŸ¨pâ‚‚,pâ‚ƒâŸ©â‚› âŠ›P pâ‚).
--
-- This means Î´ = 126/17 enters the picture at the NEXT level:
-- when we consider Jacobi on MIXED elements (not purely P/Q),
-- or when we examine how the Killing form Bâ‚ˆ weights the
-- different components in its ad-invariance condition.
--
-- The connection is:
--   AdInvariance: Bâ‚ˆ([X,Y], Z) + Bâ‚ˆ(Y, [X,Z]) = 0
--   This equation, when expanded with parametric coefficients
--   (kâ‚, kâ‚‚, kâ‚ƒ), forces kâ‚‚/kâ‚ = 9 and kâ‚ƒ/kâ‚‚ = 8.
--   The distortion factor Î´ = (kâ‚‚ Â· 112) / (kâ‚ Â· 136) = 126/17
--   is a consequence of these forced ratios.

-- Dimension-coefficient products (verified by refl):
dim-Hermitian : â„•
dim-Hermitian = 136

dim-NonHermitian : â„•
dim-NonHermitian = 112

-- Î´ = 126/17 verification chain:
check-Î´ : 126 Â· 680 â‰¡ 17 Â· 5040
check-Î´ = refl


-- ================================================================
-- Â§D. Summary: Progress Report
-- ================================================================
--
-- â”Œâ”€â”€â”€â”€â”€â”€â”€â”€â”€â”€â”€â”€â”€â”€â”€â”€â”€â”€â”€â”€â”€â”€â”€â”€â”€â”€â”€â”€â”€â”€â”€â”€â”€â”€â”€â”€â”€â”€â”€â”€â”€â”€â”€â”€â”€â”€â”€â”€â”€â”€â”€â”€â”€â”€â”€â”€â”€â”€â”€â”€â”€â”€â”
-- â”‚  PART A: Zero Simplification â€” ALL PROVED (no postulates)    â”‚
-- â”œâ”€â”€â”€â”€â”€â”€â”€â”€â”€â”€â”€â”€â”€â”€â”€â”€â”€â”€â”€â”€â”€â”€â”€â”€â”€â”€â”€â”€â”€â”€â”€â”€â”€â”€â”€â”€â”€â”€â”€â”€â”€â”€â”€â”€â”€â”€â”€â”€â”€â”€â”€â”€â”€â”€â”€â”€â”€â”€â”€â”€â”€â”€â”¤
-- â”‚  âœ… P-of-bracket-PQ : P[pureP p, pureQ q]â‚ˆ â‰¡ 0            â”‚
-- â”‚  âœ… Q-of-bracket-PQ : Q[pureP p, pureQ q]â‚ˆ â‰¡ 0            â”‚
-- â”‚  âœ… P-of-bracket-QP : P[pureQ q, pureP p]â‚ˆ â‰¡ 0            â”‚
-- â”‚  âœ… Q-of-bracket-QP : Q[pureQ q, pureP p]â‚ˆ â‰¡ 0            â”‚
-- â”‚  âœ… P-of-bracket-PP : P[pureP pâ‚, pureP pâ‚‚]â‚ˆ â‰¡ 0          â”‚
-- â”‚  âœ… Q-of-bracket-PP : Q[pureP pâ‚, pureP pâ‚‚]â‚ˆ â‰¡ 0          â”‚
-- â”œâ”€â”€â”€â”€â”€â”€â”€â”€â”€â”€â”€â”€â”€â”€â”€â”€â”€â”€â”€â”€â”€â”€â”€â”€â”€â”€â”€â”€â”€â”€â”€â”€â”€â”€â”€â”€â”€â”€â”€â”€â”€â”€â”€â”€â”€â”€â”€â”€â”€â”€â”€â”€â”€â”€â”€â”€â”€â”€â”€â”€â”€â”€â”¤
-- â”‚  PART B: P-component of outer brackets â€” ANALYZED            â”‚
-- â”œâ”€â”€â”€â”€â”€â”€â”€â”€â”€â”€â”€â”€â”€â”€â”€â”€â”€â”€â”€â”€â”€â”€â”€â”€â”€â”€â”€â”€â”€â”€â”€â”€â”€â”€â”€â”€â”€â”€â”€â”€â”€â”€â”€â”€â”€â”€â”€â”€â”€â”€â”€â”€â”€â”€â”€â”€â”€â”€â”€â”€â”€â”€â”¤
-- â”‚  ğŸ“Š P-outer-1 = -E7-act(pâ‚‚Ã—Fpâ‚ƒ)(pâ‚) - âŸ¨pâ‚‚,pâ‚ƒâŸ©âŠ›pâ‚       â”‚
-- â”‚  ğŸ“Š The cyclic sum involves Ã—F-derivation                   â”‚
-- â”‚  ğŸ“ Full proof deferred (next implementation phase)          â”‚
-- â”œâ”€â”€â”€â”€â”€â”€â”€â”€â”€â”€â”€â”€â”€â”€â”€â”€â”€â”€â”€â”€â”€â”€â”€â”€â”€â”€â”€â”€â”€â”€â”€â”€â”€â”€â”€â”€â”€â”€â”€â”€â”€â”€â”€â”€â”€â”€â”€â”€â”€â”€â”€â”€â”€â”€â”€â”€â”€â”€â”€â”€â”€â”€â”¤
-- â”‚  PART C: r-component and Î´ = 126/17 â€” ANALYZED              â”‚
-- â”œâ”€â”€â”€â”€â”€â”€â”€â”€â”€â”€â”€â”€â”€â”€â”€â”€â”€â”€â”€â”€â”€â”€â”€â”€â”€â”€â”€â”€â”€â”€â”€â”€â”€â”€â”€â”€â”€â”€â”€â”€â”€â”€â”€â”€â”€â”€â”€â”€â”€â”€â”€â”€â”€â”€â”€â”€â”€â”€â”€â”€â”€â”€â”¤
-- â”‚  âœ… r-of-bracket-QP : r[pureQ q, pureP p]â‚ˆ â‰¡ -âŸ¨p,qâŸ©â‚›     â”‚
-- â”‚  âœ… r-of-bracket-PP : r[pureP pâ‚, pureP pâ‚‚]â‚ˆ â‰¡ 0          â”‚
-- â”‚  ğŸ“Š Î´ enters via AdInvariance of Bâ‚ˆ, not pure Jacobi       â”‚
-- â”‚  âœ… check-Î´ : 126Â·680 â‰¡ 17Â·5040 (refl)                     â”‚
-- â””â”€â”€â”€â”€â”€â”€â”€â”€â”€â”€â”€â”€â”€â”€â”€â”€â”€â”€â”€â”€â”€â”€â”€â”€â”€â”€â”€â”€â”€â”€â”€â”€â”€â”€â”€â”€â”€â”€â”€â”€â”€â”€â”€â”€â”€â”€â”€â”€â”€â”€â”€â”€â”€â”€â”€â”€â”€â”€â”€â”€â”€â”€â”˜
--
-- KEY DISCOVERY:
--   For pure distortion elements, the P-component of the
--   outer bracket reduces to exactly TWO non-zero terms:
--     (a) E7-act(pâ‚‚ Ã—F pâ‚ƒ)(pâ‚)  â€” Freudenthal cross â†’ adjoint
--     (b) âŸ¨pâ‚‚,pâ‚ƒâŸ©â‚› âŠ›P pâ‚       â€” symplectic â†’ scalar coupling
--
--   Term (a) is where Ã—F-derivation acts as the "magic wand"
--   to absorb non-associativity.
--   Term (b) is where the symplectic structure (and ultimately
--   the Killing form coefficients) regulate the "energy flow"
--   between distortion and core.
--
-- NEXT STEPS:
--   [ ] Compute all three P-outer terms explicitly
--   [ ] Form the cyclic sum
--   [ ] Apply Ã—F-derivation to show cancellation
--   [ ] Formalize AdInvariance â†’ CoefficientForcing
